examples/POPLmark.v
@@ -7,15 +7,15 @@ Inductive type : Type :=
 | Arr (A1 A2 : type)
 | All (A1 : type) (A2 : {bind type}).
 
-Instance VarConstr_type : VarConstr type. derive_VarConstr. Defined.
-Instance Rename_type : Rename type. derive_Rename. Defined.
-Instance Subst_type : Subst type. derive_Subst. Defined.
+Instance VarConstr_type : VarConstr type. derive. Defined.
+Instance Rename_type : Rename type. derive. Defined.
+Instance Subst_type : Subst type. derive. Defined.
 
-Instance SubstLemmas_type : SubstLemmas type. derive_SubstLemmas. Qed.
+Instance SubstLemmas_type : SubstLemmas type. derive. Qed.
 
 Instance size_type : Size type. 
 assert(Size var). exact(fun _ => 0).
-derive_Size. Defined.
+derive. Defined.
 
 Inductive term :=
 | TeVar (x : var)
@@ -24,24 +24,22 @@ Inductive term :=
 | TAbs (A : type) (s : {bind type in term})
 | TApp (s : term) (A : type).
 
-Instance hsubst_term : HSubst type term. derive_HSubst. Defined.
+Instance hsubst_term : HSubst type term. derive. Defined.
 
 
-Instance VarConstr_term : VarConstr term. derive_VarConstr. Defined.
-Instance Rename_term : Rename term. derive_Rename. Defined.
-Instance Subst_term : Subst term. derive_Subst. Defined.
+Instance VarConstr_term : VarConstr term. derive. Defined.
+Instance Rename_term : Rename term. derive. Defined.
+Instance Subst_term : Subst term. derive. Defined.
 
-Instance HSubstLemmas_term : HSubstLemmas type term _ _ _ _. derive_HSubstLemmas. Qed.
+Instance HSubstLemmas_term : HSubstLemmas type term. derive. Qed.
 
-Instance SubstHSubstComp_type_term : SubstHSubstComp type term _ _. 
-derive_SubstHSubstComp.
-Qed.
+Instance SubstHSubstComp_type_term : SubstHSubstComp type term. derive. Qed.
 
-Instance substLemmas_term : SubstLemmas term. derive_SubstLemmas. Qed.
+Instance substLemmas_term : SubstLemmas term. derive. Qed.
 
 Instance size_term : Size term. 
 assert(Size var). exact(fun _ => 0).
-derive_Size. Defined.
+derive. Defined.
 
 Lemma ren_size_inv (A : type) : forall xi, size A.[ren xi] = size A.
 Proof.
